Top-level enc-enc conf proof. Tweaks.

verified/sec_prop.i.dfy
@@ -5,26 +5,132 @@ include "entry.s.dfy"
 //-----------------------------------------------------------------------------
 // Enclave-Enclave Confidentiality
 //-----------------------------------------------------------------------------
+predicate ni_reqs(s1: state, d1: PageDb, s1': state, d1': PageDb,
+                  s2: state, d2: PageDb, s2': state, d2': PageDb,
+                  atkr: PageNr)
+{
+    SaneState(s1) && validPageDb(d1) && SaneState(s1') && validPageDb(d1') &&
+    SaneState(s2) && validPageDb(d2) && SaneState(s2') && validPageDb(d2') &&
+    pageDbCorresponds(s1.m, d1) && pageDbCorresponds(s1'.m, d1') &&
+    pageDbCorresponds(s2.m, d2) && pageDbCorresponds(s2'.m, d2') &&
+    valDispPage(d1, atkr) && valDispPage(d2, atkr)
+}
+
+predicate ni_reqs_(d1: PageDb, d1': PageDb, d2: PageDb, d2': PageDb, atkr: PageNr)
+{
+    validPageDb(d1) && validPageDb(d1') &&
+    validPageDb(d2) && validPageDb(d2') &&
+    valDispPage(d1, atkr) && valDispPage(d2, atkr)
+}
+
+predicate same_call_args(s1:state, s2: state)
+    requires SaneState(s1) && SaneState(s2)
+{
+    reveal_ValidRegState();
+    reveal_ValidSRegState();
+    OperandContents(s1, OReg(R0))  == OperandContents(s2, OReg(R0)) &&
+    OperandContents(s1, OReg(R1))  == OperandContents(s2, OReg(R1)) &&
+    OperandContents(s1, OReg(R2))  == OperandContents(s2, OReg(R2)) &&
+    OperandContents(s1, OReg(R3))  == OperandContents(s2, OReg(R3)) &&
+    OperandContents(s1, OReg(R4))  == OperandContents(s2, OReg(R4))
+}
+
+lemma enc_enc_conf_ni(s1: state, d1: PageDb, s1': state, d1': PageDb,
+                      s2: state, d2: PageDb, s2': state, d2': PageDb,
+                      atkr: PageNr)
+    requires ni_reqs(s1, d1, s1', d1', s2, d2, s2', d2', atkr)
+    requires same_call_args(s1, s2)
+    // If smchandler(s1, d1) => (s1', d1')
+    requires smchandler(s1, d1, s1', d1')
+    // and smchandler(s2, d2) => (s2', d2')
+    requires smchandler(s2, d2, s2', d2')
+    // s.t. (s1, d1) =_{atkr} (s2, d2)
+    requires enc_enc_conf_eqpdb(d1, d2, atkr)
+    requires (var callno := s1.regs[R0]; var dispPage := s1.regs[R1];
+        (callno == KOM_SMC_ENTER || callno == KOM_SMC_RESUME) && dispPage == atkr 
+            ==> enc_enc_conf_eq(s1, s2, d1, d2, atkr))
+    // then (s1', d1') =_{atkr} (s2', d2')
+    // (maybe the following line should really be valDisp(_,atkr) ==> d1 =_L d2)
+    ensures valDispPage(d1', atkr) && valDispPage(d2', atkr) &&
+        enc_enc_conf_eqpdb(d1', d2', atkr)  
+    ensures (var callno := s1.regs[R0]; var dispPage := s1.regs[R1];
+        (callno == KOM_SMC_ENTER || callno == KOM_SMC_RESUME) && dispPage == atkr 
+            ==> enc_enc_conf_eq(s1', s2', d1', d2', atkr))
+{
+    reveal_ValidRegState();
+    var callno, arg1, arg2, arg3, arg4
+        := s1.regs[R0], s1.regs[R1], s1.regs[R2], s1.regs[R3], s1.regs[R4];
+    var e1', e2' := s1'.regs[R0], s2'.regs[R0];
+
+    if(callno == KOM_SMC_QUERY){
+        assume false;
+    }
+    if(callno == KOM_SMC_GETPHYSPAGES){
+        assume false;
+    }
+    if(callno == KOM_SMC_INIT_ADDRSPACE){
+       initAddrspace_enc_enc_conf_ni(d1, d1', e1', d2, d2', e2', arg1, arg2, atkr);
+    }
+    if(callno == KOM_SMC_INIT_DISPATCHER){
+       initDispatcher_enc_enc_conf_ni(d1, d1', e1', d2, d2', e2', arg1, arg2, arg3, atkr);
+    }
+    if(callno == KOM_SMC_INIT_L2PTABLE){
+       initL2PTable_enc_enc_conf_ni(d1, d1', e1', d2, d2', e2', arg1, arg2, arg3, atkr);
+    }
+    if(callno == KOM_SMC_MAP_SECURE){
+       mapSecure_enc_enc_conf_ni(d1, d1', e1', d2, d2', e2', arg1, arg2, arg3, arg4, atkr);
+    }
+    if(callno == KOM_SMC_MAP_INSECURE){
+       mapInsecure_enc_enc_conf_ni(d1, d1', e1', d2, d2', e2', arg1, arg2, arg3, atkr);
+    }
+    if(callno == KOM_SMC_REMOVE){
+       remove_enc_enc_conf_ni(d1, d1', e1', d2, d2', e2', arg1, atkr);
+    }
+    if(callno == KOM_SMC_FINALISE){
+       finalise_enc_enc_conf_ni(d1, d1', e1', d2, d2', e2', arg1, atkr);
+    }
+    if(callno == KOM_SMC_ENTER){
+       enter_enc_enc_conf_ni(s1, d1, s1', d1', s2, d2, s2', d2', arg1, arg2, arg3, arg4, atkr);
+    }
+    if(callno == KOM_SMC_RESUME){
+       resume_enc_enc_conf_ni(s1, d1, s1', d1', s2, d2, s2', d2', arg1, atkr);
+    }
+    if(callno == KOM_SMC_STOP){
+       assume false;
+       // This guy's not happy about a precond.
+       stop_enc_enc_conf_ni(d1, d1', e1', d2, d2', e2', arg1, atkr);
+    }
+}
 
 lemma enter_enc_enc_conf_ni(s1: state, d1: PageDb, s1':state, d1': PageDb,
                             s2: state, d2: PageDb, s2':state, d2': PageDb,
-                    dispPage: word, arg1: word, arg2: word, arg3: word)
-    requires SaneState(s1) && validPageDb(d1) && SaneState(s1') && validPageDb(d1')
-    requires SaneState(s2) && validPageDb(d2) && SaneState(s2') && validPageDb(d2')
-    requires pageDbCorresponds(s1.m, d1) && pageDbCorresponds(s1'.m, d1') 
-    requires pageDbCorresponds(s2.m, d2) && pageDbCorresponds(s2'.m, d2') 
-    requires validPageNr(dispPage) && valDispPage(d1, dispPage) && 
-        valDispPage(d1', dispPage)// Error case??
-    // If smc_enter(s1, d1) => (s1', d1')
+                            dispPage: word, arg1: word, arg2: word, arg3: word,
+                            atkr: PageNr)
+    requires ni_reqs(s1, d1, s1', d1', s2, d2, s2', d2', atkr)
     requires smc_enter(s1, d1, s1', d1', dispPage, arg1, arg2, arg3)
-    // and smc_enter(s2, d2) => (s2', d2')
     requires smc_enter(s2, d2, s2', d2', dispPage, arg1, arg2, arg3)
-    // s.t. (s1, d1) =_{disp} (s2, d2)
-    requires enc_enc_conf_eqpdb(d1, d2, dispPage)
-    requires enc_enc_conf_eq(s1, s2, d1, d2, dispPage)
-    // then (s1', d1') =_{disp} (s2', d2')
-    ensures  enc_enc_conf_eqpdb(d1', d2', dispPage)
-    ensures  enc_enc_conf_eq(s1', s2', d1', d2', dispPage)
+    requires enc_enc_conf_eqpdb(d1, d2, atkr)
+    requires dispPage == atkr ==> enc_enc_conf_eq(s1, s2, d1, d2, atkr)
+    ensures  valDispPage(d1', atkr) && valDispPage(d2', atkr) &&
+        enc_enc_conf_eqpdb(d1', d2', atkr)
+    ensures  dispPage == atkr ==> enc_enc_conf_eq(s1', s2', d1', d2', atkr)
+{
+    // TODO proveme
+    assume false;
+}
+
+lemma resume_enc_enc_conf_ni(s1: state, d1: PageDb, s1':state, d1': PageDb,
+                            s2: state, d2: PageDb, s2':state, d2': PageDb,
+                            dispPage: word,
+                            atkr: PageNr)
+    requires ni_reqs(s1, d1, s1', d1', s2, d2, s2', d2', atkr)
+    requires smc_resume(s1, d1, s1', d1', dispPage)
+    requires smc_resume(s2, d2, s2', d2', dispPage)
+    requires enc_enc_conf_eqpdb(d1, d2, atkr)
+    requires dispPage == atkr ==> enc_enc_conf_eq(s1, s2, d1, d2, atkr)
+    ensures  valDispPage(d1', atkr) && valDispPage(d2', atkr) &&
+        enc_enc_conf_eqpdb(d1', d2', atkr)
+    ensures  dispPage == atkr ==> enc_enc_conf_eq(s1', s2', d1', d2', atkr)
 {
     // TODO proveme
     assume false;
@@ -33,14 +139,15 @@ lemma enter_enc_enc_conf_ni(s1: state, d1: PageDb, s1':state, d1': PageDb,
 lemma initAddrspace_enc_enc_conf_ni(d1: PageDb, d1': PageDb, e1':word,
                                     d2: PageDb, d2': PageDb, e2':word,
                                     addrspacePage:word, l1PTPage:word,
-                                    atkr: word)
-    requires validPageDb(d1) && validPageDb(d1') &&
-        validPageDb(d2) && validPageDb(d2')
-    requires validPageNr(atkr) && valDispPage(d1, atkr) && valDispPage(d2, atkr)
+                                    atkr: PageNr)
+    requires ni_reqs_(d1, d1', d2, d2', atkr)
     requires smc_initAddrspace(d1, addrspacePage, l1PTPage) == (d1', e1')
     requires smc_initAddrspace(d2, addrspacePage, l1PTPage) == (d2', e2')
     requires enc_enc_conf_eqpdb(d1, d2, atkr)
     ensures enc_enc_conf_eqpdb(d1', d2', atkr) 
+    // Not sure that the following is really needed... I don't think the 
+    // enclaves can observe the error ?
+    // If this is needed, it should be pushed to the top-level thing
     ensures (validPageNr(addrspacePage) &&
         (d1[atkr].addrspace == addrspacePage ||
             d2[atkr].addrspace == addrspacePage))
@@ -71,6 +178,104 @@ lemma initAddrspace_enc_enc_conf_ni(d1: PageDb, d1': PageDb, e1':word,
                 }
         }
     }
+}
+
+lemma initDispatcher_enc_enc_conf_ni(d1: PageDb, d1': PageDb, e1':word,
+                                     d2: PageDb, d2': PageDb, e2':word,
+                                     page:word, addrspacePage:word, entrypoint:word,
+                                     atkr: PageNr)
+    requires ni_reqs_(d1, d1', d2, d2', atkr)
+    requires smc_initDispatcher(d1, page, addrspacePage, entrypoint) == (d1', e1')
+    requires smc_initDispatcher(d2, page, addrspacePage, entrypoint) == (d2', e2')
+    requires enc_enc_conf_eqpdb(d1, d2, atkr)
+    ensures enc_enc_conf_eqpdb(d1', d2', atkr) 
+{
+    // PROVEME
+    assume false;
+}
+
+lemma initL2PTable_enc_enc_conf_ni(d1: PageDb, d1': PageDb, e1':word,
+                                   d2: PageDb, d2': PageDb, e2':word,
+                                   page:word, addrspacePage:word, l1index:word,
+                                   atkr: PageNr)
+    requires ni_reqs_(d1, d1', d2, d2', atkr)
+    requires smc_initL2PTable(d1, page, addrspacePage, l1index) == (d1', e1')
+    requires smc_initL2PTable(d2, page, addrspacePage, l1index) == (d2', e2')
+    requires enc_enc_conf_eqpdb(d1, d2, atkr)
+    ensures enc_enc_conf_eqpdb(d1', d2', atkr) 
+{
+    // PROVEME
+    assume false;
+}
+
+lemma mapSecure_enc_enc_conf_ni(d1: PageDb, d1': PageDb, e1':word,
+                                d2: PageDb, d2': PageDb, e2':word,
+                                page:word, addrspacePage:word, mapping:word, physPage: word,
+                                atkr: PageNr)
+    requires ni_reqs_(d1, d1', d2, d2', atkr)
+    requires smc_mapSecure(d1, page, addrspacePage, mapping, physPage) == (d1', e1')
+    requires smc_mapSecure(d2, page, addrspacePage, mapping, physPage) == (d2', e2')
+    requires enc_enc_conf_eqpdb(d1, d2, atkr)
+    ensures enc_enc_conf_eqpdb(d1', d2', atkr) 
+{
+    // PROVEME
+    assume false;
+}
+
+lemma mapInsecure_enc_enc_conf_ni(d1: PageDb, d1': PageDb, e1':word,
+                                  d2: PageDb, d2': PageDb, e2':word,
+                                  addrspacePage:word, physPage: word, mapping: word,
+                                  atkr: PageNr)
+    requires ni_reqs_(d1, d1', d2, d2', atkr)
+    requires smc_mapInsecure(d1, addrspacePage, physPage, mapping) == (d1', e1')
+    requires smc_mapInsecure(d2, addrspacePage, physPage, mapping) == (d2', e2')
+    requires enc_enc_conf_eqpdb(d1, d2, atkr)
+    ensures enc_enc_conf_eqpdb(d1', d2', atkr) 
+{
+    // PROVEME
+    assume false;
+}
+
+lemma remove_enc_enc_conf_ni(d1: PageDb, d1': PageDb, e1':word,
+                             d2: PageDb, d2': PageDb, e2':word,
+                             page:word,
+                             atkr: PageNr)
+    requires ni_reqs_(d1, d1', d2, d2', atkr)
+    requires smc_remove(d1, page) == (d1', e1')
+    requires smc_remove(d2, page) == (d2', e2')
+    requires enc_enc_conf_eqpdb(d1, d2, atkr)
+    ensures  page != atkr ==> enc_enc_conf_eqpdb(d1', d2', atkr) 
+{
+    // PROVEME
+    assume false;
+}
+
+lemma finalise_enc_enc_conf_ni(d1: PageDb, d1': PageDb, e1':word,
+                             d2: PageDb, d2': PageDb, e2':word,
+                             addrspacePage:word,
+                             atkr: PageNr)
+    requires ni_reqs_(d1, d1', d2, d2', atkr)
+    requires smc_finalise(d1, addrspacePage) == (d1', e1')
+    requires smc_finalise(d2, addrspacePage) == (d2', e2')
+    requires enc_enc_conf_eqpdb(d1, d2, atkr)
+    ensures  enc_enc_conf_eqpdb(d1', d2', atkr) 
+{
+    // PROVEME
+    assume false;
+}
+
+lemma stop_enc_enc_conf_ni(d1: PageDb, d1': PageDb, e1':word,
+                             d2: PageDb, d2': PageDb, e2':word,
+                             addrspacePage:word,
+                             atkr: PageNr)
+    requires ni_reqs_(d1, d1', d2, d2', atkr)
+    requires smc_stop(d1, addrspacePage) == (d1', e1')
+    requires smc_stop(d2, addrspacePage) == (d2', e2')
+    requires enc_enc_conf_eqpdb(d1, d2, atkr)
+    ensures  enc_enc_conf_eqpdb(d1', d2', atkr) 
+{
+    // PROVEME
+    assume false;
 }
 
 
